\documentclass{article}
\usepackage[utf8]{inputenc}
\usepackage{amsfonts,amsmath,mathtools}
\usepackage{graphicx}
\newcommand{\indep}{\rotatebox[origin=c]{90}{$\models$}}

\title{Math 502AB - Lecture 13}
\author{Dr. Jamshidian}
\date{October 9, 2017}
\begin{document}

\maketitle

\section{Lecture - Part 1}

\subsubsection{Theorem: Conditional Variance Identity}

\begin{equation*}
    Var(Y) = Var(E[Y|X]) + E[Var(Y|X)]
\end{equation*}

Where:

\begin{equation*}
\begin{split}
    Var(E[Y|X]) &= E\left(E[Y|X] \right)^2 - \left(E(E[Y|X])\right)^2\\
    E[Var(Y|X)] &= E\left[E(Y^2|X) - (E[Y|X])^2 \right]
\end{split}
\end{equation*}


\subsubsection*{Proof:}

\begin{equation*}
\begin{split}
    Var[E(Y|X)] &= E[E(Y|X)^2] - E[Y]^2\\
    E[Var(Y|X)] &= E[E(Y^2|X)] - E[E(Y|X)]^2\\
                &= E[Y^2] - E[E(Y|X)]^2
\end{split}
\end{equation*}

If we add these two together, we get $Var(Y)$.


\subsubsection*{Example:}

Consider the Beta-binomial distribution. That is, consider:

\begin{equation*}
    \begin{split}
        X|P &\sim binomial(n,\mathcal{P})\\
        \mathcal{P} &\sim Beta(\alpha,\beta)
    \end{split}
\end{equation*}

Find the variance of $X$.

\begin{equation*}
    \begin{split}
        Var(X) &= Var[E(X|\mathcal{P})] + E[Var(X|\mathcal{P})]\\
        &= Var[n\mathcal{P}] + E[n\mathcal{P}(1-\mathcal{P})]\\
        &= n^2 Var(\mathcal{P}) + n E[\mathcal{P}] - nE[\mathcal{P}^2]\\
        &= \cdots
    \end{split}
\end{equation*}


\subsubsection*{Example}

This is \textbf{Problem 4.33} in the book. Say we have $N$ insects, where each insect lays $X_i$ \textbf{(iid)} eggs where $X_i \indep N$. We want to find $H$, the distribution of the \textit{total number of eggs}.

\begin{equation*}
    \begin{split}
        N &\sim Poisson(\lambda)\\
        X_i &\sim logarithmic(p)\\
        P(X_i=x) &= \frac{-(1-p)^x}{x\log p} \quad x = 1,2,\dots\\
        H &= X_1 + \dots + X_N | N
    \end{split}
\end{equation*}

To find $H$, we want to find the \textit{moment generating function}:
\begin{equation*}
     M_H(t) = E[e^{tH}] = E_N[E(e^{tH}|N)]
\end{equation*}

We note:
\begin{equation*}
    \begin{split}
        E[e^{tH}|N] &= E[e^{t(x_1+...+x_N)}|N]\\
                    &= \prod_{i=1}^N E[e^{tx_i}|N]\\
                    &= [E(e^{tx_1}|N)]^N\\
                E(e^{tx_1}|N) &= \sum_{x=1}^\infty e^{tx} \frac{-(1-p)^x}{x\log p}\\
                        &= -\frac{1}{\log p }\left[-\log \left(1-e^t(1-p) \right)\right]
    \end{split}
\end{equation*}

So, we have:

\begin{equation*}
    \begin{split}
        E[e^{tH}] &= E[E(e^{tH}|N)]\\
            &= E_N\left(\frac{\log(1-e^t(1-p)}{\log p} \right)^N\\
            &= \sum_{n=0}^\infty \left(\frac{\log(1-e^t(1-p)}{\log p} \right)^n \frac{e^{-\lambda} \lambda^n}{n!}\\
            &= ... \text{ (algebra)}\\
            &= \left(\frac{p}{1-e^{t(1-p)}} \right)^{-\lambda/\log p}\\
        H &\sim Neg. Binom.\left(r = -\frac{\lambda}{\log p}, p\right)
    \end{split}
\end{equation*}


\end{document}